nit

examples/layeredeffects/Test.fst
@@ -22,81 +22,95 @@ open HoareST
 
 /// Note that we don't need FStar.ST since the layered effects abstraction does not need it for verification
 
-#set-options "--max_fuel 0 --max_ifuel 0 --using_facts_from '* -FStar.ST'"
+#set-options "--max_fuel 0 --initial_ifuel 4 --max_ifuel 4 --using_facts_from '* -FStar.ST'"
 
-
-/// In this test:
-///   `3` is first lifted from `Tot` to `HoareST`
-///   and then its type is weakened to the annotated type
-
-let test ()
+assume val test (x:int)
 : HoareST int
-  (fun _ -> True)
-  (fun h0 r h1 -> r > 1 /\ h0 == h1)
-= 3
+  (fun _ -> x > 0)
+  (fun _ y _ -> y > x)
 
-/// This fails since the postcondition is incorrect
-
-[@expect_failure]
-let test_fail ()
-: HoareST int
-  (fun _ -> True)
-  (fun _ r _ -> r > 3)
-= 3
+#restart-solver
+#set-options "--log_queries"
+let test1 (l:list int)
+: HoareST int (fun _ -> True) (fun _ _ _ -> True)
+= match l with
+  | []   -> test 1
+  | hd::_ -> test hd
 
 
-/// Testing binds
 
-let test2 ()
-: HoareST int
-  (fun _ -> True)
-  (fun h0 r h1 -> r >= 4 /\ h0 == h1)
-= let x = test () in
-  let y = test () in
-  x + y
+// /// In this test:
+// ///   `3` is first lifted from `Tot` to `HoareST`
+// ///   and then its type is weakened to the annotated type
 
-let f_pure ()
-: Pure int
-  (requires True)
-  (ensures fun x -> x > 2)
-= 3
+// let test ()
+// : HoareST int
+//   (fun _ -> True)
+//   (fun h0 r h1 -> r > 1 /\ h0 == h1)
+// = 3
 
-/// More tests for bind, including lifts from Pure
+// /// This fails since the postcondition is incorrect
 
-let test3 ()
-: HoareST int
-  (fun _ -> True)
-  (fun _ r _ -> r >= 5)
-= let x = test () in
-  let y = f_pure () in
-  x + y
+// [@expect_failure]
+// let test_fail ()
+// : HoareST int
+//   (fun _ -> True)
+//   (fun _ r _ -> r > 3)
+// = 3
 
-/// This test relies on the return inserted for f_pure ()
-/// The wp of f_pure is too weak to prove the postcondition otherwise
 
-let test4 ()
-: HoareST int
-  (fun _ -> True)
-  (fun _ r _ -> r == 3)
-= let _ = test () in
-  f_pure ()
+// /// Testing binds
 
-/// This test fails if we use an alternative lift from PURE to HoareST that makes post parametric
-///   (rather than using the (~ wp (fun ...)) encoding that we use currently)
+// let test2 ()
+// : HoareST int
+//   (fun _ -> True)
+//   (fun h0 r h1 -> r >= 4 /\ h0 == h1)
+// = let x = test () in
+//   let y = test () in
+//   x + y
 
-let test5 ()
-: HoareST int
-  (fun _ -> True)
-  (fun h0 r h1 -> True)
-= let y = test () in
-  y
+// let f_pure ()
+// : Pure int
+//   (requires True)
+//   (ensures fun x -> x > 2)
+// = 3
 
-/// It relies on inserting return for f_pure
+// /// More tests for bind, including lifts from Pure
 
-let test6 ()
-: HoareST int
-  (fun _ -> True)
-  (fun _ r _ -> r == 3)
-= let x = f_pure () in
-  let y = test () in
-  x
+// let test3 ()
+// : HoareST int
+//   (fun _ -> True)
+//   (fun _ r _ -> r >= 5)
+// = let x = test () in
+//   let y = f_pure () in
+//   x + y
+
+// /// This test relies on the return inserted for f_pure ()
+// /// The wp of f_pure is too weak to prove the postcondition otherwise
+
+// let test4 ()
+// : HoareST int
+//   (fun _ -> True)
+//   (fun _ r _ -> r == 3)
+// = let _ = test () in
+//   f_pure ()
+
+// /// This test fails if we use an alternative lift from PURE to HoareST that makes post parametric
+// ///   (rather than using the (~ wp (fun ...)) encoding that we use currently)
+
+// let test5 ()
+// : HoareST int
+//   (fun _ -> True)
+//   (fun h0 r h1 -> True)
+// = let y = test () in
+//   y
+
+// /// It relies on inserting return for f_pure
+
+// let test6 ()
+// : HoareST int
+//   (fun _ -> True)
+//   (fun _ r _ -> r == 3)
+// = let x = f_pure () in
+//   let y = test () in
+//   x
